completed proof that the ->,-*,/\ fragment of LBI is undecidable

theories/BI/Utils/encoding.v
@@ -39,10 +39,9 @@ Arguments BI_ctx_hole {_ _}.
 #[local] Reserved Notation "⟦ A ⟧" (at level 0, format "⟦ A ⟧").
 #[local] Reserved Notation "Δ '--∗' φ" (at level 63, right associativity, format "Δ --∗ φ").
 
-(* The (-∗,⇒,⩑,1) fragment of LBI *)
+(* The (-∗,⇒,⩑) fragment of LBI *)
 Definition BI_fragment_impl_conj_unit c :=
   match c with
-(*  | BI_unit BI_mult => true   (* 1 *) *)
   | BI_impl _       => true   (* -∗ and ⇒ *)
   | BI_conj BI_addi => true   (* ⩑ *)
   | _               => false  (* no other connective *)
@@ -57,13 +56,13 @@ Definition BI_fragment_impl_conj_unit c :=
 
 Section pseudo_exponential.
 
-  Variable (prop : Set) (K : BI_form µ prop).
+  Variable (prop : Set) (U : BI_form µ prop).
 
-  (* We work in the (-∗,⇒,⩑,1) fragment of BI *)
+  (* We work in the (-∗,⇒,⩑) fragment of BI *)
   Implicit Types (φ : BI_form µ prop) (Γ : BI_bunch µ prop).
 
-  (* We simulate ⊤ using K⇒K *)
-  Notation "⊤" := (K⇒K).
+  (* We simulate ⊤ using U⇒U *)
+  Notation "⊤" := (U⇒U).
 
   (** This is the "major breakthrought" that allows for the encoding
       of the dereliction rule in BI, see BI_pseudo_exp_derilection below,
@@ -71,7 +70,7 @@ Section pseudo_exponential.
           The logic of bunched implications is undecidable 
           Galatos, Jipsen, Knudstorp & Ramanayake. arXiv 2026  *)
 
-  Definition BI_pseudo_exp γ φ := (⊤-∗(φ-∗γ)⇒γ)⩑K.
+  Definition BI_pseudo_exp γ φ := (⊤-∗(φ-∗γ)⇒γ) ⩑ U.
   Notation "![ γ ] φ" := (BI_pseudo_exp γ φ).
 
   (** We study the LBI proof theory of the pseudo-exponential ![γ]φ, 
@@ -80,14 +79,14 @@ Section pseudo_exponential.
   Hint Constructors LBI_provable BI_bunch_equiv : core.
   Hint Resolve LBI_neut_l : core.
 
-  (* Our encoding of ⊤ as 1⇒1 is correct *)
+  (* Our encoding of ⊤ as U⇒U is correct *)
   Local Fact LBI_top_weak Γ : Γ ⊦ ⊤.
   Proof. rule LBI_weak at []. Qed.
 
   (* The "weakening" rule for ![γ]φ *)
 
   Proposition LBI_pseudo_exp_weak Γ γ φ ψ :
-             Γ ⊛ₘ ⟨K⟩ ⊦ ψ 
+             Γ ⊛ₘ ⟨U⟩ ⊦ ψ 
       (*------------------*)
     →    Γ ⊛ₘ ⟨![γ]φ⟩ ⊦ ψ.
   Proof.
@@ -107,7 +106,7 @@ Section pseudo_exponential.
      Notice that ⨂ₘ[A₁;...;Aₙ] := A₁ ⊛ₘ (... ⊛ₘ (Aₙ ⊛ₘ 1)...) *)
   Lemma LBI_list_mult_weak Σ Γ ψ (HΣ : ∀A, A ∊ Σ → ∃ γ φ, A = ![γ]φ) :
 
-          ⨂ₘ (map (λ _, K) Σ) ⊛ₘ Γ ⊦ ψ 
+          ⨂ₘ (map (λ _, U) Σ) ⊛ₘ Γ ⊦ ψ 
     →  (*----------------------------------*)
           ⨂ₘ Σ ⊛ₘ Γ ⊦ ψ.
 
@@ -146,12 +145,12 @@ Section pseudo_exponential.
 
   Local Proposition LBI_second_idea Γ γ φ :
 
-         (Γ ⊛ₘ ⟨(⊤-∗φ)⩑K⟩) ⊛ₐ ⟨φ⟩ ⊦ γ
+         (Γ ⊛ₘ ⟨(⊤-∗φ)⩑U⟩) ⊛ₐ ⟨φ⟩ ⊦ γ
     → (*------------------------------*)
-            Γ ⊛ₘ ⟨(⊤-∗φ)⩑K⟩ ⊦ γ.
+            Γ ⊛ₘ ⟨(⊤-∗φ)⩑U⟩ ⊦ γ.
 
   Proof.
-    set (Δ := Γ ⊛ₘ ⟨(⊤-∗φ)⩑K⟩).
+    set (Δ := Γ ⊛ₘ ⟨(⊤-∗φ)⩑U⟩).
     intros H.
     apply LBI_cntr_root.
     unfold Δ at 2.
@@ -164,6 +163,7 @@ Section pseudo_exponential.
     simpl; rule LBI_impl_l at [rt].
   Qed.
 
+(*
   Definition LBI_pwith γ φ ψ := (((φ-∗γ)⇒γ)⇒((ψ-∗γ)⇒γ)⇒γ)-∗γ.
 
   Local Proposition LBI_third_idea_l Γ γ φ ψ :
@@ -195,6 +195,7 @@ Section pseudo_exponential.
     rule LBI_impl_l at [].
     apply LBI_equiv with Γ; eauto.
   Qed.
+*)
 
   Local Proposition LBI_fourth_idea Γ γ φ ψ :
       Γ ⊦ φ
@@ -209,6 +210,7 @@ Section pseudo_exponential.
     rule LBI_impl_l at [].
   Qed.
 
+(*
   (* We also need to be able to discard ⟨⊤-∗(φ-∗γ)⇒γ⟩ *)
   Local Proposition LBI_fifth_idea Γ γ φ :
            Γ ⊛ₘ ⟨⊤-∗(φ-∗γ)⇒γ⟩ ⊛ₘ ⟨φ⟩ ⊦ γ
@@ -222,6 +224,8 @@ Section pseudo_exponential.
     rule LBI_impl_l at [rt].
     now apply LBI_first_idea.
   Qed.
+
+*)
 
   Proposition LBI_pseudo_exp_derilection Γ γ φ :
 
@@ -243,7 +247,7 @@ Section pseudo_exponential.
   Lemma LBI_list_mult_derilection Σ Γ γ φ (HΣ : ![γ]φ ∊ Σ) :
 
         ⨂ₘ Σ ⊛ₘ ⟨φ⟩ ⊛ₘ Γ ⊦ γ 
-    → (*---------------*)
+    → (*--------------------*)
           ⨂ₘ Σ ⊛ₘ Γ ⊦ γ.
 
   Proof.
@@ -278,10 +282,10 @@ Section pseudo_exponential.
   Qed.
 
   (** Alternate encoding w/o ⩑/& *)
-  Local Proposition LBI_fourth_idea' Γ Δ γ φ ψ :
-      Γ ⊛ₘ Δ ⊦ φ
-    → Γ ⊛ₘ Δ ⊦ ψ
-    → Γ ⊛ₘ ⟨((φ⇒ψ⇒γ)⇒γ)-∗γ⟩ ⊛ₘ Δ ⊦ γ.
+  Local Proposition LBI_FORK_alt Γ Δ γ φ ψ :
+         Γ ⊛ₘ Δ ⊦ φ       →    Γ ⊛ₘ Δ ⊦ ψ
+    → (*----------------------------------*)
+          Γ ⊛ₘ ⟨((φ⇒ψ⇒γ)⇒γ)-∗γ⟩ ⊛ₘ Δ ⊦ γ.
   Proof.
     intros H1 H2.
     apply LBI_impl_middle; auto.
@@ -290,8 +294,8 @@ Section pseudo_exponential.
 
   Local Fact LBI_INC Γ Δ φ ψ γ :
 
-             Γ ⊛ₘ ⟨φ⟩ ⊛ₘ Δ ⊦ ψ
-    → (*----------------------*)
+           Γ ⊛ₘ ⟨φ⟩ ⊛ₘ Δ ⊦ ψ
+    → (*---------------------------*)
          Γ ⊛ₘ ⟨(φ-∗ψ)-∗γ⟩ ⊛ₘ Δ ⊦ γ.
 
   Proof.
@@ -315,9 +319,9 @@ Section pseudo_exponential.
   Qed.
 
   Local Fact LBI_STOP Γ Δ γ :
-              Γ ⊛ₘ Δ ⊦ K
+              Γ ⊛ₘ Δ ⊦ U
     → (*----------------------*)
-         Γ ⊛ₘ ⟨K-∗γ⟩ ⊛ₘ Δ ⊦ γ.
+         Γ ⊛ₘ ⟨U-∗γ⟩ ⊛ₘ Δ ⊦ γ.
 
   Proof. intros; apply LBI_impl_middle; auto. Qed.
 
@@ -355,18 +359,15 @@ Section pseudo_exponential.
   Notation "⟦ A ⟧" := (tps_BI_form plus e s A).
 
   (* Semantically, ![γ]φ behaves much like φ⩑1 wrt TPS,
-     when K is interpreted the same way as 1
+     when U is interpreted the same way as 1
      hence irrelevant of the choice of γ *)
-  Proposition tps_BI_pseudo_exp γ φ : (∀x, ⟦K⟧ x ↔ e = x) → ⟦φ⟧ e → ∀x, ⟦![γ]φ⟧ x ↔ e = x.
+  Proposition tps_BI_pseudo_exp γ φ : ⟦U⟧ e → ⟦φ⟧ e→ ⟦![γ]φ⟧ e.
   Proof using comm neut.
-    intros HK Hφ x; split.
-    1: intros []; apply HK; auto.
-    intros <-.
-    split; [ | ].
-    + intros x _ H.
-      rewrite comm, neut in H.
-      rewrite comm; apply H; auto.
-    + now apply HK.
+    intros HU Hφ; split; auto.
+    intros x _ H.
+    rewrite comm in H |- *. 
+    rewrite neut in H.
+    now apply H.
   Qed. 
 
 End pseudo_exponential.
@@ -401,12 +402,12 @@ Section ACM2_to_BI.
   
   Abbreviation α := true.
   Abbreviation β := false.
-  Abbreviation K := (£(inl (inr tt))).
-  Notation L x := (£(inl (inl x))).
+  Abbreviation U := (£(inl (inr tt))).
+  Abbreviation L x := (£(inl (inl x))).
 
   (** This is a "positive" encoding of 2-ACM in
       the (⩑,-∗) linear fragment of BI (ie IMLL)
-        FORKₐ p q r --> q⩑r -∗ p
+        FORKₐ p q r --> ((q⇒r⇒p)⇒p) -∗ p
         INCₐ α p q  --> (α -∗ q) -∗ p
         DECₐ β p q  --> β -∗ q -∗ p
         STOPₐ p     --> K -∗ p
@@ -418,14 +419,14 @@ Section ACM2_to_BI.
       
   Definition acm2_instr_to_BI i : BI_form µ ((loc+unit)+bool) :=
     match i with
-    | FORKₐ p q r => (L q ⩑ L r) -∗ L p
+    | FORKₐ p q r => ((L q ⇒ L r ⇒ L p) ⇒ L p) -∗ L p
     | INCₐ c p q  => (£(inr c) -∗ L q) -∗ L p
     | DECₐ c p q  => £(inr c) -∗ L q -∗ L p
-    | STOPₐ p     => K -∗ L p
+    | STOPₐ p     => U -∗ L p
     end.
 
   Abbreviation encᵢ := acm2_instr_to_BI.
-  Notation "![ γ ] φ" := (BI_pseudo_exp K γ φ).
+  Notation "![ γ ] φ" := (BI_pseudo_exp U γ φ).
   
   Definition acm2_code_to_BI := list_prod (λ p i, ![L p](encᵢ i)) l Σ.
 
@@ -478,7 +479,7 @@ Section ACM2_to_BI.
 
   Notation "Δ --∗ φ" := (BI_multi_wand Δ φ).
 
-  Definition acm2_to_BI x y p := ((map (λ _, K) acm2_code_to_BI)--∗K)⇒enc x y--∗(L p).
+  Definition acm2_to_BI x y p := (acm2_code_to_BI--∗U)⇒enc x y--∗(L p).
 
   (** We can now show that our positive encoding is sound
       wrt to cut-free provability in the (-∗,⇒,⩑) fragment *)
@@ -504,20 +505,18 @@ Section ACM2_to_BI.
                    ];
         match goal with
         | _ : ?i ∊ Σ |- _ => apply LBI_list_mult_derilection
-                               with (K := K) (φ := acm2_instr_to_BI i)
+                               with (U := U) (φ := acm2_instr_to_BI i)
         end; auto; simpl acm2_instr_to_BI.
     + apply LBI_STOP.
       unfold enc; simpl.
-      apply LBI_list_mult_weak with K.
-      1: intros A (k & i & -> & [])%list_prod_spec; eauto.
-      (* we show K^n ⊛ₘ (K^n --∗K) ⊦ K *)
+      (* we show U^n ⊛ₘ (U^n --∗U) ⊦ U *)
       induction acm2_code_to_BI as [ | ? m IH]; simpl.
-      * apply LBI_equiv with ⟨K⟩; auto.
+      * apply LBI_equiv with ⟨U⟩; auto.
       * apply LBI_middle_move.
         rule LBI_impl_l at [lft].
         revert IH; apply LBI_equiv.
         apply BI_bequiv_comm.
-    + apply LBI_FORK; auto.
+    + apply LBI_FORK_alt; auto.
     + apply LBI_INC.
       revert IH; apply LBI_equiv; auto.
     + apply LBI_INC.
@@ -549,10 +548,25 @@ Section ACM2_to_BI.
 
     Notation "⟦ A ⟧" := (tps_BI_form pair_add (0,0) tps A).
 
-    Fact tps_map_K m : ⟦map (λ _ : BI_form µ (loc + unit + bool), K) m--∗K⟧ (0, 0).
+    Fact tps_BI_zero_multi_wand Δ A : (∀B, B ∊ Δ → ⟦B⟧ ⊆ eq (0,0)) → ⟦A⟧ ⊆ ⟦Δ--∗A⟧.
     Proof.
-      induction m; simpl; auto.
-      intros ? <-; simpl; auto.
+      rewrite <- Forall_forall.
+      induction 1 as [ | B Δ H1 H2 IH2 ]; simpl; auto.
+      intros c Hc x <-%H1; apply IH2.
+      now rewrite pair_add_zero_left.
+    Qed.
+
+   Local Fact tps_BI_multi_wand_zero Δ A : (∀B, B ∊ Δ → ⟦B⟧ (0,0)) → ⟦Δ--∗A⟧ ⊆ ⟦A⟧.
+    Proof.
+      rewrite <- Forall_forall.
+      induction 1 as [ | B Δ H1 H2 IH2 ]; simpl; auto.
+      intros [] Hx;  apply IH2, (Hx _ H1).
+    Qed.
+
+    Fact tps_map_K m : ⟦map (λ _ : BI_form µ (loc + unit + bool), U) m--∗U⟧ (0, 0).
+    Proof.
+      apply tps_BI_zero_multi_wand; simpl; auto.
+      intros A (? & <- & _)%in_map_iff; auto.
     Qed.
 
     Hint Constructors acm2_accept : core.
@@ -573,7 +587,7 @@ Section ACM2_to_BI.
       + intros ? <-; simpl.
         intros []; rewrite pair_add_comm; simpl.
         now constructor 6 with q.
-      + intros [] []; rewrite pair_add_zero_right; eauto.
+      + intros []; rewrite pair_add_zero_right; unfold tps_impl; eauto.
     Qed.
 
     Local Fact tps_BI_multi_wand_α n x y A : ⟦repeat £(inr α) n--∗A⟧ (x,y) → ⟦A⟧ (n+x,y).
@@ -591,13 +605,6 @@ Section ACM2_to_BI.
       replace (S (n+y)) with (n+S y) by lia.
       apply IHn, (H _ eq_refl).
     Qed.
- 
-    Local Fact tps_BI_multi_wand_zero Δ A : (∀B, B ∊ Δ → ⟦B⟧ (0,0)) → ⟦Δ--∗A⟧ ⊆ ⟦A⟧.
-    Proof.
-      rewrite <- Forall_forall.
-      induction 1 as [ | B Δ H1 H2 IH2 ]; simpl; auto.
-      intros [] Hx;  apply IH2, (Hx _ H1).
-    Qed.
 
     Variables (x y : nat) (p : loc)
               (Hxyp : ∀c, ⟦acm2_to_BI x y p⟧ c).
@@ -606,18 +613,22 @@ Section ACM2_to_BI.
     Proof using Hxyp.
       change (tps (inl (inl p)) (x,y)).
       simpl in Hxyp.
-      specialize (Hxyp _ (tps_map_K _)).
+      Check tps_map_K.
+      specialize (Hxyp (0,0)).
       unfold tps_impl in Hxyp.
       unfold enc in Hxyp.
       rewrite !BI_mult_wand_app in Hxyp.
       apply tps_BI_multi_wand_α,
             tps_BI_multi_wand_β in Hxyp.
-      rewrite !Nat.add_0_r in Hxyp.
-      apply tps_BI_multi_wand_zero in Hxyp; auto.
-      intros B (? & i & -> & [])%list_prod_spec.
-      apply tps_BI_pseudo_exp; auto.
-      + simpl; tauto. 
-      + now apply tps_instr_sound.
+      + rewrite !Nat.add_0_r in Hxyp.
+        apply tps_BI_multi_wand_zero in Hxyp; auto.
+        intros B (? & i & -> & [])%list_prod_spec.
+        apply tps_BI_pseudo_exp; auto.
+        * now simpl.
+        * now apply tps_instr_sound.
+      + unfold acm2_code_to_BI.
+        apply tps_BI_zero_multi_wand; simpl; auto.
+        intros ? (? & ? & -> & _)%list_prod_spec ? []; auto.
     Qed.
 
   End completeness.
